src/tutorial/FiniteSimulation.v
@@ -4,6 +4,13 @@ From Tutorial Require Import Refinement.
 
 Set Implicit Arguments.
 
+(** Our goal in refinement-based verification is to prove the refines relation between the source and the target program.
+    However, refines relation is difficult to prove directly in general.
+    A standard approach is to define a relation called simulation, which simplifies the proof by enabling a *step-wise* reasoning.
+    In this file, we define a *inductive* simulation, which can be used to prove refinement between programs with *finite* executions.
+    To reason about programs which can possibly diverge, we need a coinductive simulation, which will be presented later.
+ *)
+
 Section SIM.
 
   Context {event: Event}.
@@ -12,17 +19,17 @@ Section SIM.
   Notation ekind := event.(label_kind).
   Notation sort := sem.(state_sort).
 
+  (* Inductive simulation. We only have to reason one (source or target) step at a time. *)
   Inductive sim
-            (RR: Z -> Z -> Prop)
     :
     sem.(state) -> sem.(state) -> Prop :=
   | sim_term
       st_src st_tgt r_src r_tgt
       (TERMS: sort st_src = final r_src)
       (TERMT: sort st_tgt = final r_tgt)
-      (SIM: RR r_src r_tgt)
+      (SIM: r_src = r_tgt)
     :
-    sim RR st_src st_tgt
+    sim st_src st_tgt
   | sim_obs
       st_src0 st_tgt0
       (OBSS: sort st_src0 = normal)
@@ -31,42 +38,42 @@ Section SIM.
           (sem.(step) st_tgt0 ev st_tgt1) ->
           (ekind ev = observableE) /\
           exists st_src1, (sem.(step) st_src0 ev st_src1) /\
-                       (sim RR st_src1 st_tgt1))
+                       (sim st_src1 st_tgt1))
     :
-    sim RR st_src0 st_tgt0
+    sim st_src0 st_tgt0
   | sim_silentS
       st_src0 st_tgt
       (SORT: sort st_src0 = normal)
       (SIM: exists ev st_src1,
           (sem.(step) st_src0 ev st_src1) /\
             (ekind ev = silentE) /\
-            (sim RR st_src1 st_tgt))
+            (sim st_src1 st_tgt))
     :
-    sim RR st_src0 st_tgt
+    sim st_src0 st_tgt
   | sim_silentT
       st_src st_tgt0
       (SORT: sort st_tgt0 = normal)
       (SIM: forall ev st_tgt1,
           (sem.(step) st_tgt0 ev st_tgt1) ->
           (ekind ev = silentE) /\
-          (sim RR st_src st_tgt1))
+          (sim st_src st_tgt1))
     :
-    sim RR st_src st_tgt0
+    sim st_src st_tgt0
+  (* If the source can exhibit UB, the proof is done (remember that UB is the set of all traces, thus refines any program). *)
   | sim_ub
       st_src st_tgt
       (SORT: sort st_src = undef)
     :
-    sim RR st_src st_tgt
+    sim st_src st_tgt
   .
 
-  (* Coq fails to generate a correct induction lemma. *)
+  (* Because Coq fails to generate a correct induction lemma, we need to make one. *)
   Lemma sim_ind2
-        (RR: Z -> Z -> Prop)
         (P: sem.(state) -> sem.(state) -> Prop)
         (TERM: forall st_src st_tgt r_src r_tgt
                  (TERMS: sort st_src = final r_src)
                  (TERMT: sort st_tgt = final r_tgt)
-                 (SIM: RR r_src r_tgt)
+                 (SIM: r_src = r_tgt)
           ,
             P st_src st_tgt)
         (OBS: forall st_src0 st_tgt0
@@ -76,7 +83,7 @@ Section SIM.
                     (sem.(step) st_tgt0 ev st_tgt1) ->
                     (ekind ev = observableE) /\
                     exists st_src1, (sem.(step) st_src0 ev st_src1) /\
-                                 (sim RR st_src1 st_tgt1) /\ (P st_src1 st_tgt1))
+                                 (sim st_src1 st_tgt1) /\ (P st_src1 st_tgt1))
           ,
             P st_src0 st_tgt0)
         (SILENTS: forall st_src0 st_tgt
@@ -84,7 +91,7 @@ Section SIM.
                     (SIM: exists ev st_src1,
                         (sem.(step) st_src0 ev st_src1) /\
                           (ekind ev = silentE) /\
-                          (sim RR st_src1 st_tgt) /\ (P st_src1 st_tgt))
+                          (sim st_src1 st_tgt) /\ (P st_src1 st_tgt))
           ,
             P st_src0 st_tgt)
         (SILENTT: forall st_src st_tgt0
@@ -92,7 +99,7 @@ Section SIM.
                     (SIM: forall ev st_tgt1,
                         (sem.(step) st_tgt0 ev st_tgt1) ->
                         (ekind ev = silentE) /\
-                        ((sim RR st_src st_tgt1) /\ (P st_src st_tgt1)))
+                        ((sim st_src st_tgt1) /\ (P st_src st_tgt1)))
           ,
             P st_src st_tgt0)
         (UB: forall st_src st_tgt
@@ -101,7 +108,7 @@ Section SIM.
             P st_src st_tgt)
     :
     forall st_src st_tgt
-      (SIM: sim RR st_src st_tgt),
+      (SIM: sim st_src st_tgt),
       P st_src st_tgt.
   Proof.
     fix IH 3. i. inv SIM.
@@ -115,19 +122,30 @@ Section SIM.
 End SIM.
 #[export] Hint Constructors sim: core.
 
+(* A complete simulation relation. *)
 Definition simulation {l: Event} {sem: @STS l} (src tgt: Program sem) :=
-  sim (@eq Z) src.(init) tgt.(init).
+  sim src.(init) tgt.(init).
+
+
+
+(** Of course, we need to prove that a simulation relation is sound, which means simulation implies refinement.
+    This sort of theorem is called an adequacy theorem.
+    The proof itself should be helpful for building an intuition behind how simulation works, so please follow the proof.
+ *)
 
 Section ADEQ.
 
   Context {event: Event}.
   Context {sem: @STS event}.
 
+  (* First prove the simulation is sound for a silent divergence case.
+     In fact, this is almost trivial because our simulation only works for finite programs, which do not divergs.
+     However, if the source can exhibit UB, the target can diverge because UB is the set of all trace.
+   *)
   Lemma adequacy_spin
-        (RR: Z -> Z -> Prop)
         (st_src: sem.(state))
         (st_tgt: sem.(state))
-        (SIM: sim RR st_src st_tgt)
+        (SIM: sim st_src st_tgt)
         (SPIN: diverge st_tgt)
     :
     diverge st_src.
@@ -146,10 +164,11 @@ Section ADEQ.
     { pfold. econs 2. auto. }
   Qed.
 
+  (* Proof for the rest of the cases is basically a proof by induction on the simulation. *)
   Lemma adequacy_aux
         (st_src0: sem.(state))
         (st_tgt0: sem.(state))
-        (SIM: sim eq st_src0 st_tgt0)
+        (SIM: sim st_src0 st_tgt0)
     :
     forall tr, (behavior st_tgt0 tr) -> (behavior st_src0 tr).
   Proof.
