README.md
@@ -1,7 +1,14 @@
 # refinement-tutorial
-Tutorial for refinement-based verification
+Tutorial for refinement-based verification.
 
 Work In Progress.
+
+Some helpful references:
+
+A convenient technique for stuttering simulation:
+Minki Cho, Youngju Song, Dongjae Lee, Lennard Gäher, and Derek Dreyer. 2023. Stuttering for Free. Proc. ACM Program. Lang. 7, OOPSLA2, Article 281 (October 2023), 28 pages. https://doi.org/10.1145/3622857.
+
+Paco: A Coq Library for Parameterized Coinduction (https://plv.mpi-sws.org/paco/).
 
 ## Build
 Requirement: opam (>=2.0.0), Coq 8.15.0
@@ -29,4 +36,4 @@ All the files are in `src/tutorial/`.
 
 -> `Simulation.v`
 
--> `Example3.v`
+-> `Example3.v` (WIP)
